Source/Concurrency/MoverCheck.cs
@@ -10,6 +10,12 @@ namespace Microsoft.Boogie
     {
       public int layer;
       public IEnumerable<Expr> extraAssumptions;
+      public HashSet<Variable> UsedGlobalVars()
+      {
+        var usedGlobalVars = new HashSet<Variable>();
+        extraAssumptions.ForEach(expr => usedGlobalVars.UnionWith(VariableCollector.Collect(expr).Where(x => x is GlobalVariable)));
+        return usedGlobalVars;
+      }
     }
 
     CivlTypeChecker civlTypeChecker;
@@ -49,25 +55,68 @@ namespace Microsoft.Boogie
         from first in civlTypeChecker.MoverActions
         from second in civlTypeChecker.MoverActions
         where first.LayerRange.OverlapsWith(second.LayerRange)
-        where first.IsRightMover || second.IsLeftMover
+        where first.IsRightMover || second.IsUnconditionalLeftMover
         select new {first, second};
-
       foreach (var moverCheck in regularMoverChecks)
       {
         if (moverCheck.first.IsRightMover)
         {
           moverChecking.CreateRightMoverCheckers(moverCheck.first, moverCheck.second);
         }
-
-        if (moverCheck.second.IsLeftMover)
+        if (moverCheck.second.IsUnconditionalLeftMover)
         {
           moverChecking.CreateLeftMoverCheckers(moverCheck.first, moverCheck.second);
         }
       }
 
-      foreach (var action in civlTypeChecker.MoverActions.Where(a => a.IsLeftMover))
+      var conditionalMoverChecks =
+        from first in civlTypeChecker.MoverActions
+        from second in civlTypeChecker.MoverActions
+        where first.LayerRange.OverlapsWith(second.LayerRange)
+        where second.IsConditionalLeftMover
+        select new {first, second};
+      foreach (var moverCheck in conditionalMoverChecks)
       {
-        moverChecking.CreateNonblockingChecker(action);
+        var leftMover = moverCheck.second;
+        var layer = leftMover.ActionDecl.LayerRange.UpperLayer;
+        var action = moverCheck.first;
+        var subst1 = Substituter.SubstitutionFromDictionary(
+            leftMover.ActionDecl.InParams.Zip(leftMover.SecondImpl.InParams.Select(x => (Expr)Expr.Ident(x))).ToDictionary(x => x.Item1, x => x.Item2));
+        var moverCheckContext1 = new MoverCheckContext
+        {
+          layer = layer,
+          extraAssumptions = leftMover.Preconditions(layer, subst1).Select(assertCmd => assertCmd.Expr),
+        };
+        var subst2 = Substituter.SubstitutionFromDictionary(
+            leftMover.ActionDecl.InParams.Zip(leftMover.FirstImpl.InParams.Select(x => (Expr)Expr.Ident(x))).ToDictionary(x => x.Item1, x => x.Item2));
+        var moverCheckContext2 = new MoverCheckContext
+        {
+          layer = layer,
+          extraAssumptions = leftMover.Preconditions(layer, subst2).Select(assertCmd => assertCmd.Expr),
+        };
+        moverChecking.CreateCommutativityChecker(action, leftMover, moverCheckContext1);
+        moverChecking.CreateGatePreservationChecker(leftMover, action, moverCheckContext2);
+        moverChecking.CreateFailurePreservationChecker(action, leftMover, moverCheckContext1);
+      }
+
+      foreach (var leftMover in civlTypeChecker.MoverActions.Where(a => a.IsLeftMover))
+      {
+        if (leftMover.IsUnconditionalLeftMover)
+        {
+          moverChecking.CreateNonblockingChecker(leftMover);
+        }
+        else
+        {
+          var layer = leftMover.ActionDecl.LayerRange.UpperLayer;
+          var subst = Substituter.SubstitutionFromDictionary(
+              leftMover.ActionDecl.InParams.Zip(leftMover.Impl.InParams.Select(x => (Expr)Expr.Ident(x))).ToDictionary(x => x.Item1, x => x.Item2));
+          var moverCheckContext = new MoverCheckContext
+          {
+            layer = layer,
+            extraAssumptions = leftMover.Preconditions(layer, subst).Select(assertCmd => assertCmd.Expr),
+          };
+          moverChecking.CreateNonblockingChecker(leftMover, moverCheckContext);
+        }
       }
 
       /*
@@ -106,7 +155,7 @@ namespace Microsoft.Boogie
             var moverCheckContext = new MoverCheckContext
             {
               layer = sequentialization.Layer,
-              extraAssumptions = sequentialization.Preconditions(leftMover, subst).Select(assertCmd => assertCmd.Expr)
+              extraAssumptions = leftMover.Preconditions(sequentialization.Layer, subst).Select(assertCmd => assertCmd.Expr)
             };
             moverChecking.CreateNonblockingChecker(leftMover, moverCheckContext);
           }
@@ -191,6 +240,10 @@ namespace Microsoft.Boogie
       frame.UnionWith(first.UsedGlobalVarsInAction);
       frame.UnionWith(second.UsedGlobalVarsInGate);
       frame.UnionWith(second.UsedGlobalVarsInAction);
+      if (moverCheckContext != null)
+      {
+        frame.UnionWith(moverCheckContext.UsedGlobalVars());
+      }
 
       var linearTypeChecker = civlTypeChecker.linearTypeChecker;
       List<Requires> requires =
@@ -262,6 +315,10 @@ namespace Microsoft.Boogie
       frame.UnionWith(first.UsedGlobalVarsInGate);
       frame.UnionWith(second.UsedGlobalVarsInGate);
       frame.UnionWith(second.UsedGlobalVarsInAction);
+      if (moverCheckContext != null)
+      {
+        frame.UnionWith(moverCheckContext.UsedGlobalVars());
+      }
 
       var linearTypeChecker = civlTypeChecker.linearTypeChecker;
       List<Requires> requires = 
@@ -323,6 +380,10 @@ namespace Microsoft.Boogie
       frame.UnionWith(first.UsedGlobalVarsInGate);
       frame.UnionWith(second.UsedGlobalVarsInGate);
       frame.UnionWith(second.UsedGlobalVarsInAction);
+      if (moverCheckContext != null)
+      {
+        frame.UnionWith(moverCheckContext.UsedGlobalVars());
+      }
 
       var linearTypeChecker = civlTypeChecker.linearTypeChecker;
       List<Requires> requires = 
@@ -386,6 +447,10 @@ namespace Microsoft.Boogie
       HashSet<Variable> frame = new HashSet<Variable>();
       frame.UnionWith(action.UsedGlobalVarsInGate);
       frame.UnionWith(action.UsedGlobalVarsInAction);
+      if (moverCheckContext != null)
+      {
+        frame.UnionWith(moverCheckContext.UsedGlobalVars());
+      }
 
       List<Requires> requires =
         DisjointnessAndWellFormedRequires(impl.InParams.Where(v => LinearTypeChecker.FindLinearKind(v) != LinearKind.LINEAR_OUT),
